disk-betree/ImplModelFlushPolicy.i.dfy
@@ -284,6 +284,7 @@ module ImplModelFlushPolicy {
   requires Inv(k, s)
   requires io.IOInit?
   requires s.Ready?
+  requires |s.ephemeralIndirectionTable.graph| <= IndirectionTableModel.MaxSize() - 3
   requires BT.G.Root() in s.cache
   {
     var s0 := s.(lru := LruModel.Use(s.lru, BT.G.Root()));
@@ -331,6 +332,7 @@ module ImplModelFlushPolicy {
   requires s.Ready?
   requires BT.G.Root() in s.cache
   requires runFlushPolicy(k, s, io, s', io')
+  requires |s.ephemeralIndirectionTable.graph| <= IndirectionTableModel.MaxSize() - 3
   ensures WFVars(s')
   ensures M.Next(Ik(k), IVars(s), IVars(s'), UI.NoOp, diskOp(io'))
   {
